comments on oraclehybrid

src/FCF/OracleHybrid.v
@@ -19,7 +19,8 @@ Section OracleHybrid.
   Hypothesis O2_wf : forall s a, well_formed_comp (O2 s a).
 
   (* The "adversary" that attempts to distinguish the oracles using at most q queries. *)
-  Variable A1 : OracleComp A B bool.
+  Variable A1 : OracleComp A B bool. (* TODO why an oraclecomp? review the setup *)
+  (* TODO meaning it takes an oracle of type ^ (and an initial state?), does queries on it, and returns a bool *)
   Hypothesis A1_wf : well_formed_oc A1.
   Variable q : nat.
   Hypothesis A1_qam : queries_at_most A1 q.
@@ -36,28 +37,61 @@ Section OracleHybrid.
     [b, _] <-$2 A1 _ _ O2 s;
     ret b.
 
-  (* The ith oracle responds to the first (i-1) queries using O1, and the remaining queries using O2. *)
-  Definition Oi (i : nat)(s : (State * nat))(a : A) : Comp (B * (State * nat)) :=
-    [s_s, s_i] <-2 s;
+  (* The ith oracle responds to the first (i-1) queries using O1, and the remaining queries using O2. (its state is augmented with a nat for countdown) -- where is the countdown? *)
+  Definition Oi (i : nat) (s : (State * nat)) (a : A) : Comp (B * (State * nat)) :=
+    [s_s, s_i] <-2 s;           (* just tuple notation *)
     let O_c := if (ge_dec s_i i) then O2 else O1 in
+    (* if i < s_i then O1 else O2 *)
     [b, s_s'] <-$2 O_c s_s a;
-      ret (b, (s_s', (S s_i))).
-      
-  
+      ret (b, (s_s', (S s_i))). (* s_i + 1 *)
+
+  (* TODO why does the ith game use the ith oracle? why can't the ith game directly respond to the first (i-1) queries using O1, and the remaining queries using O2?
+
+oh, because it needs to give the oracle to the adversary
+i seem to be confused about games vs. oracles, TODO rewrite
+
+How do we go through i games? There's no induction here?
+
+So G1 = G_0 = (Gi q) and G2 = G_q = (Gi 0) *)
+
+  (* TODO could the `q`s differ between games? *)
   (* The ith game uses the ith oracle.  We will show that G1 is the same as (Gi q) and that G2 is the same as (Gi 0).*)
   Definition Gi i :=
-    [b, _] <-$2 A1 _ _ (Oi i) (s, 0%nat);
+    [b, _] <-$2 A1 _ _ (Oi i) (s, 0%nat); (* what's 0 for? oh, the new overall state for Oi is (State * nat), and it increments it on each call *)
     ret b.
 
   (* We need an assumption that each adjacent pair of games are distant by at most some constant k. *)
   Variable k : Rat.
+
+  (* TODO: this is the (hard) part that we need to show? inductive hypothesis / Update? *)
   Hypothesis Gi_Si_close : 
     forall i,
-      | Pr[Gi i] - Pr[Gi (S i)] | <= k.
+  | Pr[Gi i] - Pr[Gi (S i)] | <= k. (* G_i and G_{i+1} are close *)
+
+
+  (* Our proof:
+
+G1: (assume instantiate ideal), then the adversary can query Generate+Update as many times as they want. all are done with PRF.
+
+G2: (assume instantiate ideal), then the adversary can query Generate+Update as many times as they want. all are done with random sampling.
+
+Gi i: (assume instantiate ideal), then the adversary can query Generate+Update as many times as they want (q). the first i calls are done with random sampling, the rest are done normally, with PRF.
+
+Oi: Generate+Update: modified version of PRG that does Generate n + Update with random sampling if < i, and PRF otherwise
+
+G_i_si_close: inductive hypothesis:
+
+given that K and V are randomly sampled (?),
+| Pr[G_i] - Pr[G_{i+1}] | <= PRF_advantage + Pr[collisions]
+^ more formally, what is PR[collisions]? *)
+  
 
   (* Step 1: show that G1 is the same as (Gi q).  This is actually the most complicated part of this proof. *)
 
-  (* In order to show that G1 is the same as (Gi q), we need an intermediate game that is like G1 except the oracle also keeps track of how many times it was called.  We will use an "identical until bad" proof, in which the "bad" event is that the number of queries is greater than q.  The probability of this event is 0, so we end up with an equivalence. *)
+  (* In order to show that G1 is the same as (Gi q), we need an intermediate game that is like G1 except the oracle also keeps track of how many times it was called.  
+(TODO: similar to entropy proof?)
+
+We will use an "identical until bad" proof, in which the "bad" event is that the number of queries is greater than q.  The probability of this event is 0, so we end up with an equivalence. *)
   Definition O1_count (s : (State * nat))(a : A) : Comp (B * (State * nat)) :=
     [s_s, s_i] <-2 s;
     [b, s_s'] <-$2 O1 s_s a;
@@ -157,10 +191,15 @@ Section OracleHybrid.
   Qed.
 
   (* The relational specification on O1_count and (Oi q).  As usual, I arrived at this by attempting some of the theorems below and then factoring out this theorem. *)
+  (* TODO simplify this *)
   Theorem O1_count_Oi_eq_until_bad :
-    comp_spec (fun a b => ((snd (snd a) > q) <-> (snd (snd b) > q)) /\ ((snd (snd a) <= q)%nat -> (fst a = fst b /\ fst (snd a) = fst (snd b))))
-              (A1 _ _ O1_count (s, 0)%nat)
-              (A1 _ _ (Oi q) (s, 0)%nat).
+    comp_spec 
+      (fun a b => 
+         ((snd (snd a) > q) <-> (snd (snd b) > q)) 
+         /\ ((snd (snd a) <= q)%nat 
+             -> (fst a = fst b /\ fst (snd a) = fst (snd b))))
+      (A1 _ _ O1_count (s, 0)%nat)
+      (A1 _ _ (Oi q) (s, 0)%nat).
     
     eapply comp_spec_consequence.
     eapply (fcf_oracle_eq_until_bad (fun x => if (gt_dec (snd x) q) then true else false) (fun x => if (gt_dec (snd x) q) then true else false) eq); intuition; subst.
@@ -299,14 +338,23 @@ Section OracleHybrid.
   Qed.        
 
   (* Step 3: rewrite using the equalities in the previous steps, and then use some arithmetic to show that the distance between G1 and G2 is small. *)
+  (* TODO no induction here? we gave ourselves the inductive hypothesis, I think *)
   Theorem G1_G2_close : 
     | Pr[G1] - Pr[G2] | <= (q / 1) * k.
+                             (* why (q / 1) * k? because we need to cast (q:nat) to Rat *)
 
     rewrite G1_eq_Gi_q.
     rewrite G2_eq_Gi_0.
     rewrite ratDistance_comm.
-    specialize (distance_le_prod_f (fun i => Pr[Gi i])); intuition.
-
+    Check distance_le_prod_f.
+    (* Print distance_le_prod_f. *)
+    (* f is the game;  *)
+    Check S.
+    Locate distance_le_prod_f.
+    (* clear Gi_Si_close. *)
+    specialize (distance_le_prod_f (fun i => Pr[Gi i])).
+    intuition.
+    (* specialize (distance_le_prod_f (fun i => Pr[Gi i])); intuition. *)
   Qed.
 
 End OracleHybrid.
